Progress in main encoding theorems.

mm.v
@@ -31,21 +31,19 @@ Context (Q : Type).
 Inductive mm_sym : Type :=
   | mm_a : mm_sym
   | mm_b : mm_sym
-  | mm_q : Q → mm_sym
-  | mm_c : bool → mm_sym.
+  | mm_q : Q → mm_sym.
 
 End MMSym.
 
 Arguments mm_a {Q}.
 Arguments mm_b {Q}.
 Arguments mm_q {Q} _.
-Arguments mm_c {Q} _.
 
 Section MMSymInstances.
 
-Context {Q : Type} `{!EqDecision Q}.
+Context {Q : Type}.
 
-Global Instance mm_sym_eq_dec : EqDecision (mm_sym Q).
+Global Instance mm_sym_eq_dec  `{!EqDecision Q} : EqDecision (mm_sym Q).
 Proof. solve_decision. Defined.
 
 Global Instance mm_sym_equiv : Equiv (mm_sym Q) := eq.
@@ -66,23 +64,18 @@ Context {Q : Type} `{!EqDecision Q, !Finite Q}.
 (** We construct Finite (mm_sym Q) via a bijection
     with the sum type bool + Q + bool. *)
 
-Definition mm_sym_to_sum (x : mm_sym Q) :
-    bool + bool + Q + bool :=
+Definition mm_sym_to_sum (x : mm_sym Q) : bool + Q :=
   match x with
-  | mm_a => inl (inl (inl true))
-  | mm_b => inl (inl (inl false))
-  | mm_q q => inl (inr q)
-  | mm_c b => inr b
+  | mm_a => inl true
+  | mm_b => inl false
+  | mm_q q => inr q
   end.
 
-Definition mm_sym_of_sum
-    (x : bool + bool + Q + bool) : mm_sym Q :=
+Definition mm_sym_of_sum (x : bool + Q) : mm_sym Q :=
   match x with
-  | inl (inl (inl true)) => mm_a
-  | inl (inl (inl false)) => mm_b
-  | inl (inl (inr b)) => mm_c b
-  | inl (inr q) => mm_q q
-  | inr b => mm_c b
+  | inl true => mm_a
+  | inl false => mm_b
+  | inr q => mm_q q
   end.
 
 Lemma mm_sym_of_to_sum x :
@@ -109,26 +102,25 @@ Section MMInstr.
 Context (Q : Type).
 
 Inductive mm_instr : Type :=
-  | mm_inc_a : Q → mm_instr
-  | mm_inc_b : Q → mm_instr
-  | mm_if_a : Q → Q → mm_instr
-  | mm_if_b : Q → Q → mm_instr
-  | mm_halt : bool → mm_instr.
+  | mm_inc_a : mm_instr
+  | mm_inc_b : mm_instr
+  | mm_dec_a : Q → mm_instr
+  | mm_dec_b : Q → mm_instr.
 
 End MMInstr.
 
-Arguments mm_inc_a {Q} _.
-Arguments mm_inc_b {Q} _.
-Arguments mm_if_a {Q} _ _.
-Arguments mm_if_b {Q} _ _.
-Arguments mm_halt {Q} _.
+Arguments mm_inc_a {Q}.
+Arguments mm_inc_b {Q}.
+Arguments mm_dec_a {Q} _.
+Arguments mm_dec_b {Q} _.
 
 (** ** Encoding of instructions as KA terms (Definition 13) *)
 
 Section MMEncoding.
 
 Context {Q : Type} `{!EqDecision Q, !Finite Q}.
-Implicit Types (x : mm_sym Q).
+Implicit Types (q : Q) (x : mm_sym Q).
+Variable next : Q → Q.
 
 (** Helper terms for left/right/diagonal embeddings
     (Definition 12). *)
@@ -140,27 +132,26 @@ Definition sym_r x :=
   Unit ([] : list (mm_sym Q), [x]).
 
 Definition star_d x :=
-  ka_term_diag (star (Unit [x])).
+  star (Unit ([x], [x])).
 
 (** Instruction encoding (Definition 13). *)
 
-Definition encode_instr (i : mm_instr Q) :=
+Definition encode_instr q (i : mm_instr Q) :=
   match i with
-  | mm_inc_a q =>
-      sym_r mm_a ⋅ star_d mm_a ⋅ star_d mm_b
-        ⋅ sym_r (mm_q q)
-  | mm_inc_b q =>
-      star_d mm_a ⋅ sym_r mm_b ⋅ star_d mm_b
-        ⋅ sym_r (mm_q q)
-  | mm_if_a q1 q2 =>
-      (star_d mm_b ⋅ sym_r (mm_q q1))
-      ⊔ (sym_l mm_a ⋅ star_d mm_a ⋅ star_d mm_b
-          ⋅ sym_r (mm_q q2))
-  | mm_if_b q1 q2 =>
-      (star_d mm_a ⋅ sym_r (mm_q q1))
-      ⊔ (star_d mm_a ⋅ sym_l mm_b ⋅ star_d mm_b
-          ⋅ sym_r (mm_q q2))
-  | mm_halt b => sym_r (mm_c b)
+  | mm_inc_a =>
+      sym_r mm_a ⋅ star_d mm_a ⋅ star_d mm_b ⋅
+      sym_l (mm_q q) ⋅ sym_r (mm_q (next q))
+  | mm_inc_b =>
+      star_d mm_a ⋅ sym_r mm_b ⋅ star_d mm_b ⋅
+      sym_l (mm_q q) ⋅ sym_r (mm_q (next q))
+  | mm_dec_a q' =>
+      (star_d mm_b ⋅ sym_l (mm_q q) ⋅ sym_r (mm_q (next q)))
+      ⊔ (sym_l mm_a ⋅ star_d mm_a ⋅ star_d mm_b ⋅
+         sym_l (mm_q q) ⋅ sym_r (mm_q q'))
+  | mm_dec_b q' =>
+      (star_d mm_a ⋅ sym_l (mm_q q) ⋅ sym_r (mm_q (next q)))
+      ⊔ (star_d mm_a ⋅ sym_l mm_b ⋅ star_d mm_b ⋅
+         sym_l (mm_q q) ⋅ sym_r (mm_q q'))
   end.
 
 (** Transition relation R_M (Definition 13).
@@ -168,9 +159,8 @@ Definition encode_instr (i : mm_instr Q) :=
     R_M = ⨆_{q ∈ states} encode_instr(prog q) ⋅ sym_l(q) *)
 
 Definition transition_rel (prog : Q → mm_instr Q) (states : list Q)
-    : ka_term _ :=
-  ⨆ q ∈ states,
-    encode_instr (prog q) ⋅ sym_l (mm_q q).
+    : ka_term (list (mm_sym Q) * list (mm_sym Q)) :=
+  ⨆ q ∈ states, encode_instr q (prog q).
 
 (** ** Configurations (Definition 11) *)
 
@@ -181,638 +171,254 @@ Definition config_word (ac bc : nat) (q : Q) :=
   repeat mm_a ac ++ repeat mm_b bc ++ [mm_q q].
 
 (** Configuration set C_M as a KA term:
-    C_M = (mm_a)* ⋅ (mm_b)* ⋅ ⨆_{q ∈ states} Unit [mm_q q] *)
+    C_{M,S} = (mm_a)* ⋅ (mm_b)* ⋅ ⨆_{q ∈ S} Unit [mm_q q] *)
 
-Definition config_set (states : list Q) :=
-  star (Unit [mm_a])
-    ⋅ star (Unit [mm_b])
-    ⋅ (⨆ q ∈ states, Unit [mm_q q]).
-
-(** Total configuration set T_M = C_M ⊔ {c0, c1} *)
-
-Definition total_config_set (states : list Q) :=
-  config_set states
-    ⊔ Unit [mm_c false] ⊔ Unit [mm_c true].
+Definition config_set (S : list Q) :=
+  star (Unit [mm_a]) ⋅ star (Unit [mm_b]) ⋅ ⨆ q ∈ S, Unit [mm_q q].
 
 End MMEncoding.
 
 (** ** Connection to the MM2 library *)
 
+Section Fin.
+
+(** Convert a nat to fin (S n) if in range, else 0. *)
+
+Fixpoint nat_to_fin {m} (i : nat) : option (fin m) :=
+  match m with
+  | 0 => None
+  | S m => match i with
+           | 0 => Some Fin.F1
+           | S i => Fin.FS <$> @nat_to_fin m i
+           end
+  end.
+
+Lemma nat_to_finK {m} (i : nat) (n : fin m) :
+  nat_to_fin i = Some n → fin_to_nat n = i.
+Proof.
+elim: m => //= m IH in n i *; case: i => [[<-]|] // i.
+case e: (nat_to_fin i) =>  [n'|] //= [<-] /=; congr S.
+exact: IH.
+Qed.
+
+End Fin.
+
 Section MM2Adapter.
 
 Variable P : list mm2_instr.
 Let n := length P.
-
-(** Convert a nat to fin (S n) if in range, else 0. *)
-
-Definition nat_to_fin (i : nat) : fin (S n) :=
-  match decide (i < S n) with
-  | left H => Fin.of_nat_lt H
-  | right _ => 0%fin
-  end.
+Let Q := fin (S (S n)).
 
 (** Convert a library mm2_instr at PC index i (1-indexed)
     to our mm_instr type.  Jump targets outside 1..n cause
     halting. *)
 
-Definition mm2_to_instr
-    (instr : mm2_instr) (i : nat) :
-    mm_instr (fin (S n)) :=
-  match instr with
-  | mm2_inc_a => mm_inc_a (nat_to_fin (1 + i))
-  | mm2_inc_b => mm_inc_b (nat_to_fin (1 + i))
+Definition translate_state (q : nat) : Q :=
+  match q with
+  | 0 =>
+    Fin.F1
+  | S q =>
+    Fin.FS match @nat_to_fin n q with
+           | Some q => Fin.FS q
+           | None => Fin.F1
+           end
+  end.
+
+Definition next_state (q : Q) : Q :=
+  translate_state (S q).
+
+Definition mm2_atom_fun (ρ : mm2_instr) (s : mm2_state) :=
+  let '(i,(a,b)) := s in
+  match ρ with
+  | mm2_inc_a => (1+i,(S a,b))
+  | mm2_inc_b => (1+i,(a,S b))
   | mm2_dec_a j =>
-      mm_if_a (nat_to_fin (1 + i)) (nat_to_fin j)
+    match a with
+    | 0 => (j,(0,b))
+    | S a => (1+i,(a,b))
+    end
   | mm2_dec_b j =>
-      mm_if_b (nat_to_fin (1 + i)) (nat_to_fin j)
+    match b with
+    | 0 => (j,(a,0))
+    | S b => (1+i,(a,b))
+    end
+  end.
+
+Lemma mm2_atom_fun_spec ρ s1 s2 :
+  mm2_atom ρ s1 s2 ↔ mm2_atom_fun ρ s1 = s2.
+Proof. Admitted.
+
+Arguments mm2_atom_fun_spec {_ _ _}.
+
+Definition mm2_step_fun s :=
+  match s.1 with
+  | 0 => None
+  | S i => match nth_error P i with
+           | Some ρ => Some (mm2_atom_fun ρ s)
+           | None => None
+           end
+  end.
+
+Lemma mm2_step_fun_spec s1 s2 :
+  mm2_step P s1 s2 ↔ mm2_step_fun s1 = Some s2.
+Proof. Admitted.
+
+Arguments mm2_step_fun_spec {_ _}.
+
+Definition mm2_to_instr (instr : mm2_instr) : mm_instr Q :=
+  match instr with
+  | mm2_inc_a => mm_inc_a
+  | mm2_inc_b => mm_inc_b
+  | mm2_dec_a q' => mm_dec_a (translate_state q')
+  | mm2_dec_b q' => mm_dec_b (translate_state q')
   end.
 
 (** The program function: given a state (fin (S n)),
     return the corresponding instruction.  State 0 and
     out-of-range states halt with output false. *)
 
-Definition mm2_prog (q : fin (S n)) :
-    mm_instr (fin (S n)) :=
-  match nth_error P (fin_to_nat q - 1) with
-  | Some instr => mm2_to_instr instr (fin_to_nat q)
-  | None => mm_halt false
+Definition mm2_prog (q : Q) : mm_instr Q :=
+  match nth_error P (fin_to_nat q - 2) with
+  | Some instr => mm2_to_instr instr
+  | None => mm_inc_a (* Unused *)
   end.
 
 (** Active states: all fin (S n) except 0. *)
 
-Definition active_states : list (fin (S n)) :=
-  filter (λ q, bool_decide (fin_to_nat q ≠ 0))
-         (enum (fin (S n))).
+Definition active_states : list Q :=
+  Fin.FS <$> (Fin.FS <$> enum (fin n)).
+
+(** Running configurations *)
+
+Definition C := config_set active_states.
+
+(** All configurations *)
+
+Definition T := config_set (enum Q).
+
+(** Running or accepted *)
+
+Definition partially_accepted :=
+  C ⊔ Unit (config_word 0 0 Fin.F1).
 
 (** The transition relation for a concrete MM2 program. *)
 
-Definition mm2_R := transition_rel mm2_prog active_states.
+Definition mm2_R := transition_rel next_state mm2_prog active_states.
 
 (** Encode an MM2 state as a configuration word. *)
 
-Definition mm2_config (s : mm2_state) :
-    list (mm_sym (fin (S n))) :=
-  config_word (fst (snd s)) (snd (snd s))
-              (nat_to_fin (fst s)).
+Definition mm2_config (s : mm2_state) : list (mm_sym Q) :=
+  config_word (fst (snd s)) (snd (snd s)) (translate_state (fst s)).
+
+Lemma elem_of_C s : Unit (mm2_config s) ⊑ C ↔ 0 < s.1 ≤ n.
+Proof. Admitted.
+
+Lemma elem_of_T s : Unit (mm2_config s) ⊑ T.
+Proof. Admitted.
+
+(** ** The encoding faithfully represents the transitions of a Minsky machine (~
+Lemma 14). *)
+
+Lemma encoding_complete s1 s2 :
+  mm2_step P s1 s2 →
+  Unit (mm2_config s1, mm2_config s2) ⊑ mm2_R.
+Proof. Admitted.
+
+Lemma encoding_sound s1 w :
+  Unit (mm2_config s1, w) ⊑ mm2_R →
+  ∃ s2, w = mm2_config s2 ∧ mm2_step P s1 s2.
+Proof. Admitted.
+
+Lemma encoding_rtc_complete s1 s2 :
+  rtc (mm2_step P) s1 s2 →
+  rtc (λ xs ys, Unit (xs, ys) ⊑ mm2_R) (mm2_config s1) (mm2_config s2).
+Proof. Admitted.
+
+Lemma encoding_rtc_sound s1 ys :
+  rtc (λ xs ys, Unit (xs, ys) ⊑ mm2_R) (mm2_config s1) ys →
+  ∃ s2, ys = mm2_config s2 ∧ rtc (mm2_step P) s1 s2.
+Proof. Admitted.
+
+Lemma mm2_R_ub1 : ka_term_proj1 mm2_R ⊑ T.
+Proof. Admitted.
+
+Lemma mm2_R_ub2 : ka_term_proj2 mm2_R ⊑ T.
+Proof. Admitted.
+
+Lemma repr_rel_mm2_R : repr_rel (pad_rel mm2_R) (pad_lang T).
+Proof.
+apply: bounded_output_repr_rel'.
+- apply: finite_state_join_list => q active_q.
+  by case: (mm2_prog q) => //= *; apply: finite_stateP.
+- apply: bounded_output_join_list => q active_q.
+  by case: (mm2_prog q) => //= *; apply: bounded_outputbP.
+- exact: mm2_R_ub1.
+- exact: mm2_R_ub2.
+Qed.
+
+Definition red_lb s1 :=
+  Unit (1, map Some (mm2_config s1) ⋅ [None]) ⋅ star (pad_rel mm2_R).
+
+Definition red_ub :=
+  dpseudo_top ⋅ ka_term_inj2 (pad_lang partially_accepted)
+  ⊔ repr_rel_rtc_error repr_rel_mm2_R.
+
+Lemma mm2_R_soundness_aux s1 s2 :
+  rtc (mm2_step P) s1 s2 →
+  red_lb s1 ⊑ red_ub →
+  s2 = (0,(0,0)) ∨ 0 < s2.1 ≤ n.
+Proof.
+rewrite /red_ub /repr_rel_rtc_error -assoc.
+move=> /encoding_rtc_complete s1_s2 ub.
+have pa: Unit (mm2_config s2) ⊑ partially_accepted.
+{ exact: repr_rel_rtc_soundness' s1_s2 ub. }
+rewrite -elem_of_C comm -!l_alt /= in pa *; case: pa => pa; eauto.
+right; move/leibniz_equiv_iff: pa; rewrite /mm2_config /config_word /=.
+by case: (s2) => [[|?] [[|?] [|?]]] //=.
+Qed.
+
+Lemma mm2_stop_spec s : mm2_stop P s ↔ ¬ (0 < index s ≤ n).
+Proof.
+case: s=> [i [a b]]; split.
+- move=> s_stop s_bounds; case e: (mm2_step_fun (i,(a,b))) => [s'|].
+  + by apply: (s_stop s'); apply/mm2_step_fun_spec.
+  + rewrite /mm2_step_fun /mm2_atom_fun /= in e s_bounds.
+    case: i {s_stop} => [|i] in e s_bounds; first lia.
+    case P_i: nth_error => [ρ|] //= in e *.
+    move/nth_error_None in P_i; lia.
+- move=> /= s_bounds s' /mm2_step_fun_spec.
+  rewrite /mm2_step_fun /mm2_atom_fun /=.
+  case: i => [|i] //= in s_bounds *.
+  case P_i: nth_error => [ρ|] //.
+  have: i < n by apply/nth_error_Some; congruence.
+  lia.
+Qed.
+
+Lemma mm2_R_soundness s1 s2 :
+  rtc (mm2_step P) s1 s2 →
+  mm2_stop P s2 →
+  red_lb s1 ⊑ red_ub →
+  s2 = (0,(0,0)).
+Proof.
+move=> s1_s2 /mm2_stop_spec s2_stop red_leq.
+have [//|] := mm2_R_soundness_aux s1_s2 red_leq.
+congruence.
+Qed.
+
+Lemma mm2_R_completeness s1 :
+  rtc (mm2_step P) s1 (0,(0,0)) →
+  red_lb s1 ⊑ red_ub.
+Proof.
+move=> /encoding_rtc_complete /pad_rel_rtc_1 /rtc_nsteps [m xs_ys].
+have s1_T: Unit (mm2_config s1) ⊑ T by exact: elem_of_T.
+have term: next_iter repr_rel_mm2_R (S m) [map Some (mm2_config s1) ⋅ [None]] = [].
+{ admit. }
+have := repr_rel_iter_empty' s1_T term.
+rewrite strings_r_alt; set X := next_lt _ _ _ => red_leq.
+apply: transitivity red_leq _; apply: join_mono => //.
+apply: pre_ka_mul_mono => //.
+apply: semi_lattice_morphism_sqsubseteq_proper.
+admit.
+Admitted.
 
 End MM2Adapter.
-
-(** ** Lemma 14: R_M is a partial function on configs *)
-
-Section Functional.
-
-Context {Q : Type} `{!EqDecision Q, !Finite Q}.
-Variable prog : Q → mm_instr Q.
-Variable states : list Q.
-Implicit Types (w : list (mm_sym Q)).
-Let R := transition_rel prog states.
-
-
-(** The step function computes the unique successor
-    configuration, if any. *)
-
-Definition step_config (ac bc : nat) (q : Q) :
-    option (list (mm_sym Q)) :=
-  match prog q with
-  | mm_inc_a q' =>
-      Some (config_word (S ac) bc q')
-  | mm_inc_b q' =>
-      Some (config_word ac (S bc) q')
-  | mm_if_a q1 q2 =>
-      match ac with
-      | 0 => Some (config_word 0 bc q1)
-      | S ac' => Some (config_word ac' bc q2)
-      end
-  | mm_if_b q1 q2 =>
-      match bc with
-      | 0 => Some (config_word ac 0 q1)
-      | S bc' => Some (config_word ac bc' q2)
-      end
-  | mm_halt b => Some [mm_c b]
-  end.
-
-(** Each instruction encoding, when applied to a
-    configuration, yields exactly one successor.
-
-    Unit(config_word ac bc q, w) ⊑ R  iff
-    q ∈ states and w = step_config ac bc q. *)
-
-Lemma config_in_encode_instr ac bc q w :
-  q ∈ states →
-  Unit (config_word ac bc q, w) ⊑ R →
-  step_config ac bc q = Some w.
-Proof.
-Admitted.
-
-Lemma encode_instr_config ac bc q :
-  q ∈ states →
-  ∀ w, step_config ac bc q = Some w →
-  Unit (config_word ac bc q, w) ⊑ R.
-Proof.
-move=> Hq w.
-have list_mul_app : ∀ (a b : list (mm_sym Q)),
-    a ⋅ b = a ++ b by [].
-have repeat_power : ∀ (x : mm_sym Q) n,
-    repeat x n = @power (list_monoid _) [x] n.
-{ move=> x; elim=> [|n IH] //=.
-  by rewrite -IH list_mul_app. }
-have power_le_star :
-    ∀ (T : pre_ka) (x : T) n, x ^ n ⊑ star x.
-{ move=> T' x; elim=> [|n IH] /=.
-  - exact: pre_ka_one_star.
-  - etransitivity; last exact: pre_ka_mul_star.
-    by apply: pre_ka_mul_mono. }
-have star_d_repeat : ∀ (x : mm_sym Q) n,
-    Unit (repeat x n, repeat x n)
-    ⊑ star_d x.
-{ move=> x n. rewrite /star_d
-    pre_ka_morphism_star /=.
-  elim: n => [|n IH] /=.
-  - exact: pre_ka_one_star.
-  - have -> : (x :: repeat x n, x :: repeat x n)
-      = ([x], [x]) ⋅ (repeat x n, repeat x n)
-      by [].
-    rewrite monoid_morphism_mul.
-    etransitivity; last exact: pre_ka_mul_star.
-    by apply: pre_ka_mul_mono. }
-move=> Hw0.
-rewrite /R /transition_rel.
-etransitivity; last
-  exact: sqsubseteq_join_list
-    (fun q => encode_instr (prog q)
-      ⋅ sym_l (mm_q q)) _ _ Hq.
-move: Hw0; rewrite /step_config /config_word.
-case: (prog q)=> [q'|q'|q1 q2|q1 q2|b].
-- (* mm_inc_a q' *)
-  move=> [<-].
-  have -> : (repeat mm_a ac
-    ++ repeat mm_b bc ++ [mm_q q],
-    repeat mm_a (S ac)
-    ++ repeat mm_b bc ++ [mm_q q'])
-    = (([] : list _), [mm_a])
-      ⋅ ((repeat mm_a ac, repeat mm_a ac)
-      ⋅ ((repeat mm_b bc, repeat mm_b bc)
-      ⋅ ((([] : list _), [mm_q q'])
-      ⋅ ([mm_q q], ([] : list _))))).
-  { done. }
-  rewrite !monoid_morphism_mul !assoc
-    /encode_instr /sym_r /sym_l.
-  apply: pre_ka_mul_mono;
-    [apply: pre_ka_mul_mono;
-      [apply: pre_ka_mul_mono;
-        [apply: pre_ka_mul_mono|]|]|];
-    try reflexivity; exact: star_d_repeat.
-- (* mm_inc_b q' *)
-  move=> [<-]. rewrite /config_word.
-  have -> : (repeat mm_a ac
-    ++ repeat mm_b bc ++ [mm_q q],
-    repeat mm_a ac
-    ++ repeat mm_b (S bc) ++ [mm_q q'])
-    = (repeat mm_a ac, repeat mm_a ac)
-      ⋅ ((([] : list _), [mm_b])
-      ⋅ ((repeat mm_b bc, repeat mm_b bc)
-      ⋅ ((([] : list _), [mm_q q'])
-      ⋅ ([mm_q q], ([] : list _))))).
-  { done. }
-  rewrite !monoid_morphism_mul !assoc
-    /encode_instr /sym_r /sym_l /star_d.
-  apply: pre_ka_mul_mono;
-    [apply: pre_ka_mul_mono;
-      [apply: pre_ka_mul_mono;
-        [apply: pre_ka_mul_mono|]|]|];
-    try reflexivity; exact: star_d_repeat.
-- (* mm_if_a q1 q2 *)
-  case: ac=> [|ac'].
-  + move=> [<-]. rewrite /config_word.
-    have -> :
-      (repeat mm_b bc ++ [mm_q q],
-       repeat mm_b bc ++ [mm_q q1])
-      = (repeat mm_b bc, repeat mm_b bc)
-        ⋅ ((([] : list _), [mm_q q1])
-        ⋅ ([mm_q q], ([] : list _))).
-    { rewrite /prod_mul /list_mul /=.
-      done. }
-    rewrite !monoid_morphism_mul !assoc
-      /encode_instr /sym_r /sym_l /star_d.
-    etransitivity; last
-      (apply: pre_ka_mul_mono;
-        [exact: sqsubseteq_join_left
-        |reflexivity]).
-    apply: pre_ka_mul_mono;
-      [apply: pre_ka_mul_mono|];
-      try reflexivity.
-    exact: star_d_repeat.
-  + move=> [<-]. rewrite /config_word.
-    have -> :
-      (repeat mm_a (S ac')
-        ++ repeat mm_b bc ++ [mm_q q],
-       repeat mm_a ac'
-        ++ repeat mm_b bc ++ [mm_q q2])
-      = ([mm_a], ([] : list _))
-        ⋅ ((repeat mm_a ac', repeat mm_a ac')
-        ⋅ ((repeat mm_b bc, repeat mm_b bc)
-        ⋅ ((([] : list _), [mm_q q2])
-        ⋅ ([mm_q q], ([] : list _))))).
-    { rewrite /prod_mul /list_mul /=.
-      done. }
-    rewrite !monoid_morphism_mul !assoc
-      /encode_instr /sym_r /sym_l /star_d.
-    etransitivity; last
-      (apply: pre_ka_mul_mono;
-        [exact: sqsubseteq_join_right
-        |reflexivity]).
-    apply: pre_ka_mul_mono;
-      [apply: pre_ka_mul_mono;
-        [apply: pre_ka_mul_mono;
-          [apply: pre_ka_mul_mono|]|]|];
-      try reflexivity; exact: star_d_repeat.
-- (* mm_if_b q1 q2 *)
-  case: bc=> [|bc'].
-  + move=> [<-]. rewrite /config_word.
-    have -> :
-      (repeat mm_a ac ++ [mm_q q],
-       repeat mm_a ac ++ [mm_q q1])
-      = (repeat mm_a ac, repeat mm_a ac)
-        ⋅ ((([] : list _), [mm_q q1])
-        ⋅ ([mm_q q], ([] : list _))).
-    { rewrite /prod_mul /list_mul /=.
-      done. }
-    rewrite !monoid_morphism_mul !assoc
-      /encode_instr /sym_r /sym_l /star_d.
-    etransitivity; last
-      (apply: pre_ka_mul_mono;
-        [exact: sqsubseteq_join_left
-        |reflexivity]).
-    apply: pre_ka_mul_mono;
-      [apply: pre_ka_mul_mono|];
-      try reflexivity.
-    exact: star_d_repeat.
-  + move=> [<-]. rewrite /config_word.
-    have -> :
-      (repeat mm_a ac
-        ++ repeat mm_b (S bc') ++ [mm_q q],
-       repeat mm_a ac
-        ++ repeat mm_b bc' ++ [mm_q q2])
-      = (repeat mm_a ac, repeat mm_a ac)
-        ⋅ (([mm_b], ([] : list _))
-        ⋅ ((repeat mm_b bc', repeat mm_b bc')
-        ⋅ ((([] : list _), [mm_q q2])
-        ⋅ ([mm_q q], ([] : list _))))).
-    { rewrite /prod_mul /list_mul /=.
-      done. }
-    rewrite !monoid_morphism_mul !assoc
-      /encode_instr /sym_r /sym_l /star_d.
-    etransitivity; last
-      (apply: pre_ka_mul_mono;
-        [exact: sqsubseteq_join_right
-        |reflexivity]).
-    apply: pre_ka_mul_mono;
-      [apply: pre_ka_mul_mono;
-        [apply: pre_ka_mul_mono;
-          [apply: pre_ka_mul_mono|]|]|];
-      try reflexivity; exact: star_d_repeat.
-- (* mm_halt b: encode_instr (mm_halt b) has no
-     star_d terms, so this case requires additional
-     assumptions about prog/states. *)
-  admit.
-Admitted.
-
-End Functional.
-
-(** ** Soundness helpers *)
-
-Section SoundnessHelpers.
-
-Context {Q : Type} `{!EqDecision Q, !Finite Q}.
-
-(** The nat_to_fin of a halting state's index yields
-    0%fin (which is not an active state). *)
-
-Lemma nat_to_fin_0 (P : list mm2_instr) :
-  fin_to_nat (nat_to_fin P 0) = 0.
-Proof. rewrite /nat_to_fin; by case: (decide _). Qed.
-
-Lemma nat_to_fin_oor (P : list mm2_instr) i :
-  ¬ (i < S (length P)) → nat_to_fin P i = 0%fin.
-Proof. rewrite /nat_to_fin; by case: (decide _). Qed.
-
-Lemma halt_nat_to_fin_zero (P : list mm2_instr)
-    (s : mm2_state) :
-  mm2_stop P s →
-  fin_to_nat (nat_to_fin P (fst s)) = 0.
-Proof.
-move=> Hstop.
-case E: (fst s) => [|i]; first exact: nat_to_fin_0.
-suff : nat_to_fin P (S i) = 0%fin by move=> ->.
-apply: nat_to_fin_oor => Hlt.
-have Hi : i < length P by lia.
-have Hnth : nth_error P i ≠ None
-  by rewrite nth_error_Some.
-case Heq: (nth_error P i) Hnth => [instr|] // _.
-have [xl [xr [HP Hl]]] := nth_error_split _ _ Heq.
-have Hat : mm2_instr_at instr (S i) P.
-{ exists xl, xr. split. exact HP. lia. }
-destruct s as [pc [va vb]]; simpl in E |- *.
-subst pc.
-apply: (Hstop
-  (match instr with
-   | mm2_inc_a => (2+i, (S va, vb))
-   | mm2_inc_b => (2+i, (va, S vb))
-   | mm2_dec_a j => match va with
-     | 0 => (2+i, (0, vb)) | S a => (j, (a, vb)) end
-   | mm2_dec_b j => match vb with
-     | 0 => (2+i, (va, 0)) | S b => (j, (va, b)) end
-   end)).
-exists instr; split; first exact Hat.
-case: instr {Heq HP Hl Hat Hstop} => [| |j|j].
-- exact: in_mm2s_inc_a.
-- exact: in_mm2s_inc_b.
-- case: va => [|a];
-    [exact: in_mm2s_dec_a0|exact: in_mm2s_dec_aS].
-- case: vb => [|b];
-    [exact: in_mm2s_dec_b0|exact: in_mm2s_dec_bS].
-Qed.
-
-(** Active states do not contain 0%fin. *)
-
-Lemma zero_not_active (P : list mm2_instr) :
-  ∀ q, q ∈ active_states P →
-  fin_to_nat q ≠ 0.
-Proof.
-move=> q /elem_of_list_filter [/Is_true_true Hq _].
-by move/bool_decide_eq_true: Hq.
-Qed.
-
-(** config_word with state q ∉ states is not in the
-    language of config_set states. *)
-
-Lemma config_not_in_set (ac bc : nat)
-    (q : Q) (states : list Q) :
-  q ∉ states →
-  ¬ l (config_set states) (config_word ac bc q).
-Proof.
-move=> Hq /= [w12 [w3
-  [/leibniz_equiv_iff Ewc [_ Hw3]]]].
-have /l_alt Hw3' := Hw3.
-move: (iffRL (l_alt _ _) Hw3').
-rewrite semi_lattice_morphism_join_list.
-move/elem_of_lang_join_list =>
-  [q' [Hq' /= /leibniz_equiv_iff Hw3e]].
-apply: Hq. suff -> : q = q' by [].
-have Ewc' : config_word ac bc q = w12 ++ w3
-  := Ewc.
-have := f_equal (@reverse _) Ewc'.
-rewrite Hw3e /config_word !reverse_app /=.
-by case.
-Qed.
-
-(** A config_word is never equal to [mm_c b]. *)
-
-Lemma config_word_ne_mc (ac bc : nat) (q : Q) (b : bool) :
-  config_word ac bc q ≠ [mm_c b].
-Proof.
-rewrite /config_word; case: ac => [|ac'] /=.
-- case: bc => [|bc'] /=; by discriminate.
-- by discriminate.
-Qed.
-
-(** Halting configuration is not in C ⊔ Unit [mm_c true]. *)
-
-Lemma halt_config_not_in_C (P : list mm2_instr)
-    (s : mm2_state) :
-  mm2_stop P s →
-  ¬ l (config_set (active_states P)
-       ⊔ Unit [mm_c true])
-    (mm2_config P s).
-Proof.
-move=> Hstop.
-have Hfin := halt_nat_to_fin_zero Hstop.
-rewrite /mm2_config /= => Hin.
-case: Hin => [Hc|/= /leibniz_equiv_iff Habs].
-2: { rewrite /config_word in Habs.
-     by case: (fst (snd s)) Habs => [|?] /=;
-       case: (snd (snd s)) => [|?]. }
-(* config(s) ∉ C because state is 0%fin *)
-move: Hc => /= [w12 [w3
-  [/leibniz_equiv_iff Ewc [_ Hw3]]]].
-have /l_alt Hw3' := Hw3.
-move: (iffRL (l_alt _ _) Hw3').
-rewrite semi_lattice_morphism_join_list.
-move/elem_of_lang_join_list =>
-  [q' [Hq' /= /leibniz_equiv_iff Hw3e]].
-have Hna : nat_to_fin P (fst s) ∉
-    active_states P.
-{ move=> /elem_of_list_filter
-    [/Is_true_true Hq _].
-  by move/bool_decide_eq_true: Hq;
-    rewrite Hfin. }
-apply: Hna. suff -> : nat_to_fin P (fst s) = q'
-  by [].
-have Ewc' : config_word _ _ (nat_to_fin P (fst s))
-  = w12 ++ w3 := Ewc.
-have := f_equal (@reverse _) Ewc'.
-by rewrite Hw3e /config_word !reverse_app /=
-  => [[= ->]].
-Qed.
-
-End SoundnessHelpers.
-
-Lemma fin_to_nat_of_nat_lt n m (H : n < m) :
-  fin_to_nat (@Fin.of_nat_lt n m H) = n.
-Proof.
-revert m H; induction n as [|n IH];
-  intros [|m] H; try lia; simpl; auto.
-Qed.
-
-(** Each mm2_step maps to a pair in mm2_R. *)
-
-Lemma mm2_step_in_R (P : list mm2_instr)
-    (x y : mm2_state) :
-  mm2_step P x y →
-  Unit (mm2_config P x, mm2_config P y) ⊑ mm2_R P.
-Proof.
-case=> ρ [Hat Hatom].
-rewrite /mm2_config.
-set qi := nat_to_fin P (fst x).
-have Hqi_range : 1 ≤ fst x ≤ length P.
-{ case: Hat => [l [r [HP Hl]]].
-  rewrite HP length_app /=. lia. }
-have Hqi : qi ∈ active_states P.
-{ apply/elem_of_list_filter; split;
-    last exact: elem_of_enum.
-  apply/Is_true_true/bool_decide_eq_true.
-  rewrite /qi /nat_to_fin.
-  case: (decide _) => [Hlt|]; last lia.
-  by rewrite fin_to_nat_of_nat_lt; lia. }
-have Hnth : nth_error P (fin_to_nat qi - 1)
-  = Some ρ.
-{ case: Hat => [l0 [r0 [HP Hl0]]].
-  rewrite /qi /nat_to_fin.
-  case: (decide _) => [Hlt|Hnlt]; last first.
-  { exfalso; apply: Hnlt. lia. }
-  rewrite fin_to_nat_of_nat_lt.
-  replace (fst x - 1) with (length l0) by lia.
-  rewrite HP nth_error_app2 //
-    Nat.sub_diag //. }
-Admitted.
-
-(** Building a trace pair in Unit([], config(s)) ⋅ star R.
-    After following the trace s ↠ s', there exists L such
-    that (L, L ++ config(s')) is in the LHS. *)
-
-Lemma trace_pair (P : list mm2_instr)
-    (x s' : mm2_state) :
-  P // x ↠ s' →
-  ∃ L,
-    Unit (L, L ++ mm2_config P s') ⊑
-      Unit ([], mm2_config P x) ⋅ star (mm2_R P).
-Proof.
-move=> Hrt. move: (clos_rt_rt1n _ _ _ _ Hrt)
-  => {Hrt}.
-elim.
-- move=> y; exists [].
-  rewrite -{1}[Unit _](right_id 1).
-  apply: pre_ka_mul_mono => //.
-  exact: pre_ka_one_star.
-- move=> x0 y z Hstep _ [L IH].
-  exists (mm2_config P x0 ++ L).
-  have -> :
-    (mm2_config P x0 ++ L,
-     (mm2_config P x0 ++ L) ++ mm2_config P z)
-    = ((mm2_config P x0, mm2_config P x0)
-       : list _ * list _) ⋅ (L, L ++ mm2_config P z).
-  { change ((mm2_config P x0 ++ L,
-      (mm2_config P x0 ++ L) ++ mm2_config P z)
-    = (mm2_config P x0 ⋅ L,
-       mm2_config P x0 ⋅ (L ++ mm2_config P z))).
-    by rewrite /mul /list_mul -app_assoc. }
-  rewrite monoid_morphism_mul.
-  etransitivity.
-  { apply: pre_ka_mul_mono;
-      [reflexivity | exact: IH]. }
-  rewrite assoc -monoid_morphism_mul.
-  have -> :
-    ((mm2_config P x0, mm2_config P x0)
-     : list _ * list _)
-    ⋅ (1, mm2_config P y)
-    = ((1, mm2_config P x0) : list _ * list _)
-      ⋅ (mm2_config P x0, mm2_config P y).
-  { change
-     ((mm2_config P x0 ⋅ (1 : list _),
-       mm2_config P x0 ⋅ mm2_config P y)
-     = ((1 : list _) ⋅ mm2_config P x0,
-        mm2_config P x0 ⋅ mm2_config P y)).
-    by rewrite /mul /list_mul app_nil_r. }
-  rewrite monoid_morphism_mul -assoc.
-  apply: pre_ka_mul_mono; first reflexivity.
-  etransitivity.
-  { apply: pre_ka_mul_mono;
-      [exact: mm2_step_in_R Hstep
-      | reflexivity]. }
-  exact: pre_ka_mul_star.
-Qed.
-
-(** ** Theorem 15 (Soundness) and Theorem 16 (Completeness)
-
-    These are stated for a concrete MM2 program.  The full
-    proofs require the representable-relation machinery
-    from repr_rel.v and bounded_output.v. *)
-
-Section MainTheorems.
-
-Variable P : list mm2_instr.
-Let n := length P.
-Let Q := fin (S n).
-
-(** Theorem 15 (Soundness):
-
-    If s^r ⋅ R* ⊑ Σ*_d ⋅ (C_M ⊔ c1)^r ⊔ error  in the
-    language model, then every halting computation from s
-    produces output 1 (i.e., reaches mm_c true). *)
-
-Let W : monoid :=
-  list_monoid (mm_sym_setoid (Q:=fin (S n))).
-
-Definition rhs :=
-  let C : ka_term W := config_set (active_states P) in
-  dpseudo_top ⋅ ka_term_inj2 (C ⊔ Unit [mm_c true])
-    ⊔ dpseudo_top ⋅ mismatch ⋅ pseudo_top.
-
-Theorem soundness s :
-  let R := mm2_R P in
-  l (Unit ([], mm2_config P s) ⋅ star R) ⊑ l rhs →
-  ∀ s', P // s ↠ s' →
-    mm2_stop P s' →
-    mm2_config P s' = [mm_c true].
-Proof.
-move=> R Hle s' Hreach Hstop. exfalso.
-(* Step 1: Build a trace pair (L, L ++ config(s'))
-   in the LHS language via trace_pair. *)
-have [L HL] := trace_pair Hreach.
-(* Step 2: This pair is in l(LHS), and by the
-   inequality Hle, also in l(rhs). *)
-have Hin : l rhs (L, L ++ mm2_config P s').
-{ apply: Hle. exact/l_alt. }
-(* Step 3: Decompose rhs = A ⊔ B.
-   Show (L, L ++ config(s')) is in neither A nor B.
-
-   A = dpseudo_top ⋅ ka_term_inj2(C ⊔ Unit [mm_c true]):
-     Pairs (w, w ++ t) with t ∈ C ⊔ Unit [mm_c true].
-     Our t = config(s'). Since s' is halting,
-     config(s') ∉ C (halting state 0%fin ∉ active)
-     and config(s') ≠ [mm_c true] (structurally).
-     So (L, L++config(s')) ∉ A.
-     [uses halt_config_not_in_C]
-
-   B = dpseudo_top ⋅ mismatch ⋅ pseudo_top:
-     Pairs (w++[x]++w1, w++[y]++w2) with x ≠ y.
-     Our pair has left as prefix of right, so the
-     "divergence point" would satisfy x = y.
-     So (L, L++config(s')) ∉ B.
-     [uses prefix_not_in_mismatch]
-
-   Combined: pair ∉ A ⊔ B, contradicting Hin. *)
-rewrite /rhs /= in Hin.
-case: Hin => [HA|HB].
-- change (l (dpseudo_top ⋅ ka_term_inj2
-    (config_set (active_states P)
-     ⊔ Unit [mm_c true]))
-    (L, L ++ mm2_config P s')) in HA.
-  have [suffix [Esr He]] :=
-    in_dpseudo_top_inj2 (iffLR (l_alt _ _) HA).
-  have ? : suffix = mm2_config P s'
-    by apply (app_inv_head L).
-  subst suffix.
-  exact (halt_config_not_in_C Hstop
-    (iffRL (l_alt _ _) He)).
-- change (l (dpseudo_top ⋅ mismatch ⋅ pseudo_top)
-    (L, L ++ mm2_config P s')) in HB.
-  have Hne : mm2_config P s' ≠ [].
-  { rewrite /mm2_config /config_word.
-    by case: (fst (snd s')) => [|?];
-       case: (snd (snd s')) => [|?]. }
-  exact (prefix_not_in_mismatch Hne
-    (iffLR (l_alt _ _) HB)).
-Qed.
-
-(** Theorem 16 (Completeness):
-
-    If the machine halts from s with output 1 (reaches
-    a configuration encoding mm_c true), then the KA
-    inequality holds in pre-KA. *)
-
-Theorem completeness s :
-  let R := mm2_R P in
-  let C : ka_term W := config_set (active_states P) in
-  (∃ s', P // s ↠ s' ∧ mm2_stop P s' ∧
-         mm2_config P s' = [mm_c true]) →
-  ∃ rho,
-    Unit ([] : list (mm_sym Q), mm2_config P s) ⋅ star R
-    ⊑ dpseudo_top ⋅ ka_term_inj2 (C ⊔ Unit [mm_c true])
-      ⊔ dpseudo_top ⋅ mismatch ⋅ rho.
-Proof.
-move=> R C [s' [_ [_ Habs]]].
-by exfalso; exact: config_word_ne_mc Habs.
-Qed.
-
-End MainTheorems.
